Cleanup

BertognaResponseTimeFP.v
@@ -64,7 +64,7 @@ Module ResponseTimeIterationFP.
 
     (* The schedulability test simply checks if we got a list of
        response-time bounds (i.e., if the computation did not fail). *)
-    Definition fp_schedulability_test (ts: sporadic_taskset) :=
+    Definition fp_schedulable (ts: sporadic_taskset) :=
       R_list ts != None.
     
     Section AuxiliaryLemmas.
@@ -522,139 +522,145 @@ Module ResponseTimeIterationFP.
                is_interfering_task_fp tsk higher_eq_priority tsk_other &&
                task_is_scheduled job_task sched tsk_other t) ts = num_cpus.
 
-      Definition no_deadline_missed_by (tsk: sporadic_task) :=
-        task_misses_no_deadline job_cost job_deadline job_task
-                                rate sched tsk.
+      Definition no_deadline_missed_by_task (tsk: sporadic_task) :=
+        task_misses_no_deadline job_cost job_deadline job_task rate sched tsk.
+      Definition no_deadline_missed_by_job :=
+        job_misses_no_deadline job_cost job_deadline rate sched.
 
-      (* Now we prove correctness of the schedulability test. *)
-      Lemma R_list_has_response_time_bounds :
-        forall rt_bounds tsk R,
-          R_list ts = Some rt_bounds ->
-          (tsk, R) \in rt_bounds ->
-          forall j : JobIn arr_seq,
-            job_task j = tsk ->
-            completed job_cost rate sched j (job_arrival j + R).
-      Proof.
-        rename H_valid_job_parameters into JOBPARAMS,
-               H_valid_task_parameters into TASKPARAMS,
-               H_restricted_deadlines into RESTR,
-               H_completed_jobs_dont_execute into COMP,
-               H_jobs_must_arrive_to_execute into MUSTARRIVE,
-               H_global_scheduling_invariant into INVARIANT,
-               H_sorted_ts into SORT,
-               H_transitive into TRANS,
-               H_unique_priorities into UNIQ,
-               H_total into TOTAL,
-               H_all_jobs_from_taskset into ALLJOBS,
-               H_ts_is_a_set into SET.
-        clear ALLJOBS.
+      Section HelperLemma.
         
-        unfold fp_schedulability_test, R_list in *.
-        induction ts as [| ts' tsk_i] using last_ind.
-        {
-          intros rt_bounds tsk R SOME IN.
-          by inversion SOME; subst; rewrite in_nil in IN.
-        }
-        {
-          intros rt_bounds tsk R SOME IN j JOBj.
-          destruct (lastP rt_bounds) as [| hp_bounds (tsk_lst, R_lst)];
-            first by rewrite in_nil in IN.
-          rewrite mem_rcons in_cons in IN; move: IN => /orP IN.
-          destruct IN as [LAST | BEGINNING]; last first.
+        (* The following lemma states that the response-time bounds
+           computed using R_list are valid. *)
+        Lemma R_list_has_response_time_bounds :
+          forall rt_bounds tsk R,
+            R_list ts = Some rt_bounds ->
+            (tsk, R) \in rt_bounds ->
+            forall j : JobIn arr_seq,
+              job_task j = tsk ->
+              completed job_cost rate sched j (job_arrival j + R).
+        Proof.
+          rename H_valid_job_parameters into JOBPARAMS,
+                 H_valid_task_parameters into TASKPARAMS,
+                 H_restricted_deadlines into RESTR,
+                 H_completed_jobs_dont_execute into COMP,
+                 H_jobs_must_arrive_to_execute into MUSTARRIVE,
+                 H_global_scheduling_invariant into INVARIANT,
+                 H_sorted_ts into SORT,
+                 H_transitive into TRANS,
+                 H_unique_priorities into UNIQ,
+                 H_total into TOTAL,
+                 H_all_jobs_from_taskset into ALLJOBS,
+                 H_ts_is_a_set into SET.
+          clear ALLJOBS.
+        
+          unfold fp_schedulable, R_list in *.
+          induction ts as [| ts' tsk_i] using last_ind.
           {
-            apply IHs with (rt_bounds := hp_bounds) (tsk := tsk); try (by ins).
-            by rewrite rcons_uniq in SET; move: SET => /andP [_ SET].
-            by ins; red; ins; apply TASKPARAMS; rewrite mem_rcons in_cons; apply/orP; right.
-            by ins; apply RESTR; rewrite mem_rcons in_cons; apply/orP; right.
-            by apply sorted_rcons_prefix in SORT.
-            {
-              intros tsk0 j0 t IN0 JOB0 BACK0.
-              exploit (INVARIANT tsk0 j0 t); try (by ins);
-                [by rewrite mem_rcons in_cons; apply/orP; right | intro INV].
-              rewrite -cats1 count_cat /= in INV.
-              unfold is_interfering_task_fp in INV.
-              generalize SOME; apply R_list_rcons_task in SOME; subst tsk_i; intro SOME.
-              assert (HP: higher_eq_priority tsk_lst tsk0 = false).
-              {
-                apply order_sorted_rcons with (x := tsk0) in SORT; [|by ins | by ins].
-                apply negbTE; apply/negP; unfold not; intro BUG.
-                exploit UNIQ; [by apply/andP; split; [by apply SORT | by ins] | intro EQ].
-                by rewrite rcons_uniq -EQ IN0 in SET.
-              }              
-              by rewrite HP 2!andFb 2!addn0 in INV.
-            }
-            by apply R_list_rcons_prefix in SOME.
+            intros rt_bounds tsk R SOME IN.
+            by inversion SOME; subst; rewrite in_nil in IN.
           }
           {
-            move: LAST => /eqP LAST.
-            inversion LAST as [[EQ1 EQ2]].
-            rewrite -> EQ1 in *; rewrite -> EQ2 in *; clear EQ1 EQ2 LAST.
-            generalize SOME; apply R_list_rcons_task in SOME; subst tsk_i; intro SOME.
-            generalize SOME; apply R_list_rcons_prefix in SOME; intro SOME'.
-            have BOUND := bertogna_cirinei_response_time_bound_fp.
-            unfold is_response_time_bound_of_task, job_has_completed_by in BOUND.
-            apply BOUND with (job_deadline := job_deadline) (job_task := job_task) (tsk := tsk_lst)
-                             (ts := rcons ts' tsk_lst) (hp_bounds := hp_bounds)
-                             (higher_eq_priority := higher_eq_priority); clear BOUND; try (by ins).
-            by apply R_list_unzip1 with (R := R_lst).
+           intros rt_bounds tsk R SOME IN j JOBj.
+             destruct (lastP rt_bounds) as [| hp_bounds (tsk_lst, R_lst)];
+              first by rewrite in_nil in IN.
+            rewrite mem_rcons in_cons in IN; move: IN => /orP IN.
+            destruct IN as [LAST | BEGINNING]; last first.
             {
-              intros hp_tsk R0 HP j0 JOB0.
-              apply IHs with (rt_bounds := hp_bounds) (tsk := hp_tsk); try (by ins).
+              apply IHs with (rt_bounds := hp_bounds) (tsk := tsk); try (by ins).
               by rewrite rcons_uniq in SET; move: SET => /andP [_ SET].
-              by red; ins; apply TASKPARAMS; rewrite mem_rcons in_cons; apply/orP; right.
+              by ins; red; ins; apply TASKPARAMS; rewrite mem_rcons in_cons; apply/orP; right.
               by ins; apply RESTR; rewrite mem_rcons in_cons; apply/orP; right.
               by apply sorted_rcons_prefix in SORT.
               {
-                intros tsk0 j1 t IN0 JOB1 BACK0.
-                exploit (INVARIANT tsk0 j1 t); try (by ins);
+                intros tsk0 j0 t IN0 JOB0 BACK0.
+                exploit (INVARIANT tsk0 j0 t); try (by ins);
                   [by rewrite mem_rcons in_cons; apply/orP; right | intro INV].
-                rewrite -cats1 count_cat /= addn0 in INV.
+                rewrite -cats1 count_cat /= in INV.
                 unfold is_interfering_task_fp in INV.
-                assert (NOINTERF: higher_eq_priority tsk_lst tsk0 = false).
+                generalize SOME; apply R_list_rcons_task in SOME; subst tsk_i; intro SOME.
+                assert (HP: higher_eq_priority tsk_lst tsk0 = false).
                 {
                   apply order_sorted_rcons with (x := tsk0) in SORT; [|by ins | by ins].
                   apply negbTE; apply/negP; unfold not; intro BUG.
-                  exploit UNIQ; [by apply/andP; split; [by apply BUG | by ins] | intro EQ].
-                  by rewrite rcons_uniq EQ IN0 in SET.
-                }
-                by rewrite NOINTERF 2!andFb addn0 in INV.
+                  exploit UNIQ; [by apply/andP; split; [by apply SORT | by ins] | intro EQ].
+                  by rewrite rcons_uniq -EQ IN0 in SET.
+                }              
+                by rewrite HP 2!andFb 2!addn0 in INV.
               }
-            }
-            by ins; apply R_list_ge_cost with (ts' := ts') (rt_bounds := hp_bounds).
-            by ins; apply R_list_le_deadline with (ts' := ts') (rt_bounds := hp_bounds).
-            {
-              ins; exploit (INVARIANT tsk_lst j0 t); try (by ins).
-              by rewrite mem_rcons in_cons; apply/orP; left.
+              by apply R_list_rcons_prefix in SOME.
             }
             {
-              rewrite [R_lst](R_list_rcons_response_time ts' hp_bounds tsk_lst); last by ins.
-              rewrite per_task_rta_fold.
-              apply per_task_rta_converges with (ts' := ts'); try (by ins).
+              move: LAST => /eqP LAST.
+              inversion LAST as [[EQ1 EQ2]].
+              rewrite -> EQ1 in *; rewrite -> EQ2 in *; clear EQ1 EQ2 LAST.
+              generalize SOME; apply R_list_rcons_task in SOME; subst tsk_i; intro SOME.
+              generalize SOME; apply R_list_rcons_prefix in SOME; intro SOME'.
+              have BOUND := bertogna_cirinei_response_time_bound_fp.
+              unfold is_response_time_bound_of_task, job_has_completed_by in BOUND.
+              apply BOUND with (job_deadline := job_deadline) (job_task := job_task) (tsk := tsk_lst)
+                               (ts := rcons ts' tsk_lst) (hp_bounds := hp_bounds)
+                               (higher_eq_priority := higher_eq_priority); clear BOUND; try (by ins).
+              by apply R_list_unzip1 with (R := R_lst).
               {
-                red; ins; apply TASKPARAMS.
-                by rewrite mem_rcons in_cons; apply/orP; right.
+                intros hp_tsk R0 HP j0 JOB0.
+                apply IHs with (rt_bounds := hp_bounds) (tsk := hp_tsk); try (by ins).
+                by rewrite rcons_uniq in SET; move: SET => /andP [_ SET].
+                by red; ins; apply TASKPARAMS; rewrite mem_rcons in_cons; apply/orP; right.
+                by ins; apply RESTR; rewrite mem_rcons in_cons; apply/orP; right.
+                by apply sorted_rcons_prefix in SORT.
+                {
+                  intros tsk0 j1 t IN0 JOB1 BACK0.
+                  exploit (INVARIANT tsk0 j1 t); try (by ins);
+                    [by rewrite mem_rcons in_cons; apply/orP; right | intro INV].
+                  rewrite -cats1 count_cat /= addn0 in INV.
+                  unfold is_interfering_task_fp in INV.
+                  assert (NOINTERF: higher_eq_priority tsk_lst tsk0 = false).
+                  {
+                    apply order_sorted_rcons with (x := tsk0) in SORT; [|by ins | by ins].
+                    apply negbTE; apply/negP; unfold not; intro BUG.
+                    exploit UNIQ; [by apply/andP; split; [by apply BUG | by ins] | intro EQ].
+                    by rewrite rcons_uniq EQ IN0 in SET.
+                  }
+                  by rewrite NOINTERF 2!andFb addn0 in INV.
+                }
               }
-              apply R_list_le_deadline with (ts' := rcons ts' tsk_lst)
+              by ins; apply R_list_ge_cost with (ts' := ts') (rt_bounds := hp_bounds).
+              by ins; apply R_list_le_deadline with (ts' := ts') (rt_bounds := hp_bounds).
+              {
+                ins; exploit (INVARIANT tsk_lst j0 t); try (by ins).
+                by rewrite mem_rcons in_cons; apply/orP; left.
+              }
+              {
+                rewrite [R_lst](R_list_rcons_response_time ts' hp_bounds tsk_lst); last by ins.
+                rewrite per_task_rta_fold.
+                apply per_task_rta_converges with (ts' := ts'); try (by ins).
+                {
+                  red; ins; apply TASKPARAMS.
+                  by rewrite mem_rcons in_cons; apply/orP; right.
+                }
+                apply R_list_le_deadline with (ts' := rcons ts' tsk_lst)
                                             (rt_bounds := rcons hp_bounds (tsk_lst, R_lst));
-                first by apply SOME'.
-              rewrite mem_rcons in_cons; apply/orP; left; apply/eqP.
-              f_equal; symmetry.
-              by apply R_list_rcons_response_time with (ts' := ts'). 
+                  first by apply SOME'.
+                rewrite mem_rcons in_cons; apply/orP; left; apply/eqP.
+                f_equal; symmetry.
+                by apply R_list_rcons_response_time with (ts' := ts'). 
+              }
             }
           }
-        }
-      Qed.
+        Qed.
 
-      (* Finally, we show that if the schedulability test suceeds, ...*)
-      Hypothesis H_test_passes: fp_schedulability_test ts.
+      End HelperLemma.
       
-      (*..., then no task misses its deadline. *)
+      (* If the schedulability test suceeds, ...*)
+      Hypothesis H_test_succeeds: fp_schedulable ts.
+      
+      (*..., then no task misses its deadline,... *)
       Theorem taskset_schedulable_by_fp_rta :
-        forall tsk, tsk \in ts -> no_deadline_missed_by tsk.
+        forall tsk, tsk \in ts -> no_deadline_missed_by_task tsk.
       Proof.
-        unfold no_deadline_missed_by, task_misses_no_deadline,
+        unfold no_deadline_missed_by_task, task_misses_no_deadline,
                job_misses_no_deadline, completed,
-               fp_schedulability_test,
+               fp_schedulable,
                valid_sporadic_job in *.
         rename H_valid_job_parameters into JOBPARAMS,
                H_valid_task_parameters into TASKPARAMS,
@@ -667,7 +673,7 @@ Module ResponseTimeIterationFP.
                H_unique_priorities into UNIQ,
                H_total into TOTAL,
                H_all_jobs_from_taskset into ALLJOBS,
-               H_test_passes into TEST.
+               H_test_succeeds into TEST.
 
         move => tsk INtsk j /eqP JOBtsk.
         have RLIST := (R_list_has_response_time_bounds).
@@ -691,6 +697,43 @@ Module ResponseTimeIterationFP.
         by apply COMPLETED.
       Qed.
 
+      (* ..., and the schedulability test yields safe response-time
+         bounds for each task. *)
+      Theorem fp_schedulability_test_yields_response_time_bounds :
+        forall tsk,
+          tsk \in ts ->
+          exists R,
+            R <= task_deadline tsk /\
+            forall (j: JobIn arr_seq),
+              job_task j = tsk ->
+              completed job_cost rate sched j (job_arrival j + R).
+      Proof.
+        intros tsk IN.
+        unfold fp_schedulable in *.
+        have TASKS := R_list_non_empty ts.
+        have BOUNDS := (R_list_has_response_time_bounds).
+        have DL := (R_list_le_deadline ts).
+        destruct (R_list ts) as [rt_bounds |]; last by ins.
+        exploit (TASKS rt_bounds tsk); [by ins | clear TASKS; intro EX].
+        destruct EX as [EX _]; specialize (EX IN); des.
+        exists R; split.
+          by apply DL with (rt_bounds0 := rt_bounds).
+          by ins; apply (BOUNDS rt_bounds tsk).
+      Qed.
+
+      (* For completeness, since all jobs of the arrival sequence
+         are spawned by the task set, we conclude that no job misses
+         its deadline. *)
+      Theorem jobs_schedulable_by_fp_rta :
+        forall (j: JobIn arr_seq), no_deadline_missed_by_job j.
+      Proof.
+        intros j.
+        have SCHED := taskset_schedulable_by_fp_rta.
+        unfold no_deadline_missed_by_task, task_misses_no_deadline in *.
+        apply SCHED with (tsk := job_task j); last by rewrite eq_refl.
+        by apply H_all_jobs_from_taskset.
+      Qed.
+      
     End Proof.
 
   End ResponseTimeIterationFP.
